Coq/Simplicity/StaticAnalysis.v
@@ -1,4 +1,4 @@
-Require Import PeanoNat.
+Require Import NArith.
 Require Import Util.List.
 Require Import Util.Option.
 
@@ -7,6 +7,8 @@ Require Import Simplicity.Core.
 Require Import Simplicity.BitMachine.
 Require Import Simplicity.Translate.
 Require Import Simplicity.Ty.
+
+Local Open Scope N_scope.
 
 Module StateShape.
 (* In this section we prove that executing Simplicity programs on the Bit
@@ -20,21 +22,8 @@ Definition spec {A B : Ty} (t : Term A B)  :=
 
 Lemma iden_spec {A : Ty} : spec (@iden A).
 Proof.
-intros x y; simpl.
-unfold copy, runMachine.
-destruct (Copy_chk _ _) as [[[l st] [_ ->]] |];[simpl|discriminate].
-intros Hxy; inversion_clear Hxy.
-do 2 rewrite fillContextShape_correct.
-unfold localStateShape; simpl.
-rewrite fullWriteFrame_size.
-reflexivity.
-Qed.
-
-Lemma unit_spec {A : Ty} : spec (@unit A).
-Proof.
-intros x y Hxy.
-inversion_clear Hxy.
-reflexivity.
+unfold spec.
+apply stateShape_copy.
 Qed.
 
 Lemma comp_spec {A B C : Ty} (s : Term A B) (t : Term B C) :
@@ -62,27 +51,25 @@ inversion_clear Ht.
 reflexivity.
 Qed.
 
+Lemma unit_spec {A : Ty} : spec (@unit A).
+Proof.
+intros x y Hxy.
+inversion_clear Hxy.
+reflexivity.
+Qed.
+
 Lemma injl_spec {A B C : Ty} (t : Term A B) :
  spec t -> spec (@injl A B C t).
 Proof.
 intros ht x y; cbn.
 repeat rewrite runMachine_seq.
-unfold write, runMachine at 3.
-destruct (Write_chk _) as [[ctx ->] |];[cbn|discriminate].
-set (x0 := fillContext _ _).
-replace (stateShape _) with (stateShape x0).
- unfold skip, runMachine at 2.
- destruct (Skip_chk _ _) as [[ctx0 ->] |];[cbn|discriminate].
- intros Hx1.
- rewrite <- (ht _ _ Hx1); clear y ht Hx1.
- do 2 rewrite fillContextShape_correct.
- unfold localStateShape; simpl.
- rewrite fullWriteFrame_size, repeat_length.
- reflexivity.
-unfold x0; do 2 rewrite fillContextShape_correct.
-unfold localStateShape; simpl.
-rewrite fullWriteFrame_size.
-reflexivity.
+assert (Hx := stateShape_write false x).
+destruct (runMachine _ x) as [x0|];[cbn|discriminate].
+rewrite (Hx _ (refl_equal _)); clear -ht.
+assert (Hx0 := stateShape_skip (padL B C) x0).
+destruct (runMachine _ x0) as [x1|];[cbn|discriminate].
+rewrite (Hx0 _ (refl_equal _)); clear -ht.
+auto.
 Qed.
 
 Lemma injr_spec {A B C : Ty} (t : Term A C) :
@@ -90,22 +77,13 @@ Lemma injr_spec {A B C : Ty} (t : Term A C) :
 Proof.
 intros ht x y; cbn.
 repeat rewrite runMachine_seq.
-unfold write, runMachine at 3.
-destruct (Write_chk _) as [[ctx ->] |];[cbn|discriminate].
-set (x0 := fillContext _ _).
-replace (stateShape _) with (stateShape x0).
- unfold skip, runMachine at 2.
- destruct (Skip_chk _ _) as [[ctx0 ->] |];[cbn|discriminate].
- intros Hx1.
- rewrite <- (ht _ _ Hx1); clear y ht Hx1.
- do 2 rewrite fillContextShape_correct.
- unfold localStateShape; simpl.
- rewrite fullWriteFrame_size, repeat_length.
- reflexivity.
-unfold x0; do 2 rewrite fillContextShape_correct.
-unfold localStateShape; simpl.
-rewrite fullWriteFrame_size.
-reflexivity.
+assert (Hx := stateShape_write true x).
+destruct (runMachine _ x) as [x0|];[cbn|discriminate].
+rewrite (Hx _ (refl_equal _)); clear -ht.
+assert (Hx0 := stateShape_skip (padR B C) x0).
+destruct (runMachine _ x0) as [x1|];[cbn|discriminate].
+rewrite (Hx0 _ (refl_equal _)); clear -ht.
+auto.
 Qed.
 
 Lemma bump_spec {A B : Ty} (t : Term A B) n (Ht : spec t) x y :
@@ -114,20 +92,18 @@ Lemma bump_spec {A B : Ty} (t : Term A B) n (Ht : spec t) x y :
 Proof.
 unfold bump.
 repeat rewrite runMachine_seq.
-unfold fwd, runMachine at 3.
-destruct (Fwd_chk _) as [[[l0 st0] [_ ->]] |];[cbn|discriminate].
-set (x1 := fillReadFrame _ _); specialize (Ht x1).
-destruct (runMachine _ x1) as [y0|];[cbn|discriminate].
+assert (Hx := stateShape_fwd n x).
+destruct (runMachine _ x) as [x0|];[cbn|discriminate].
+rewrite (Hx _ (refl_equal _)); clear -Ht.
+specialize (Ht x0).
+destruct (runMachine _ x0) as [y0|];[cbn|discriminate].
 specialize (Ht _ (refl_equal _)).
-unfold bwd, runMachine.
-destruct (Bwd_chk _) as [[[l1 st1] [_ ->]] |];[cbn|discriminate].
+assert (Hy := stateShape_bwd n y0).
+destruct (runMachine _ y0) as [y1|];[cbn|discriminate].
+specialize (Hy _ (refl_equal _)).
 intros Hxy.
-inversion_clear Hxy.
-unfold x1 in *; clear x1.
-repeat rewrite fillReadFrameShape_correct in *.
-cbn in *.
-do 2 rewrite rev_length, Nat.add_0_r in Ht.
-assumption.
+inversion Hxy.
+congruence.
 Qed.
 
 Lemma case_spec {A B C D : Ty} (s : Term (A * C) D) (t : Term (B * C) D) :
@@ -180,8 +156,267 @@ Qed.
 
 End StateShape.
 
+Module MaximumMemory.
 
+Definition extraMemoryBound : Core.Algebra := Core.Pack (Core.Class.Class (fun A B => N)
+  (fun A => 0)
+  (fun A B C s t => N.of_nat (bitSize B) + N.max s t)
+  (fun A => 0)
+  (fun A B C t => t)
+  (fun A B C t => t)
+  (fun A B C D s t => N.max s t)
+  (fun A B C s t => N.max s t)
+  (fun A B C t => t)
+  (fun A B C t => t)
+).
 
+Definition MemoryBound {A B : Ty} (t : Term A B) x : N := stateSize x + (@Core.eval _ _ t extraMemoryBound).
 
+Definition spec {A B : Ty} (t : Term A B)  :=
+  forall x n, programMaximumMemoryResidence (@Core.eval _ _ t Naive.translate) x = Some n ->
+              n <= MemoryBound t x.
 
+Lemma iden_spec {A : Ty} : spec (@iden A).
+Proof.
+intros x n; cbn.
+rewrite pMMR_copy.
+destruct (runMachine _ x) as [x0|];[cbn|discriminate].
+inversion_clear 1.
+unfold MemoryBound; cbn.
+rewrite N.add_0_r.
+reflexivity.
+Qed.
 
+Lemma comp_spec {A B C : Ty} (s : Term A B) (t : Term B C) :
+ spec s -> spec t -> spec (comp s t) .
+Proof.
+intros Hs Ht x n; cbn.
+repeat rewrite pMMR_seq.
+repeat rewrite runMachine_seq.
+cbn.
+set (x0 := Build_State _ _ _ _).
+specialize (Hs x0).
+destruct (programMaximumMemoryResidence _ x0) as [nx|];[cbn|discriminate].
+specialize (Hs _ (refl_equal _)).
+assert (Hsx := StateShape.Core_spec s x0).
+destruct (runMachine _ x0) as [y|];[cbn|discriminate].
+specialize (Hsx _ (refl_equal _)).
+rewrite pMMR_moveFrame.
+unfold moveFrame, runMachine at 2 3 4.
+destruct (MoveFrame_chk y) as [[[l ctx] ->] |];[cbn|discriminate].
+set (y0 := Build_State _ _ _ _).
+set (y := Build_State _ _ _ _) in Hsx |- *.
+specialize (Ht y0).
+destruct (programMaximumMemoryResidence _ y0) as [ny|];[cbn|discriminate].
+specialize (Ht _ (refl_equal _)).
+assert (Hty := StateShape.Core_spec t y0).
+destruct (runMachine _ y0) as [z|];[cbn|discriminate].
+specialize (Hty _ (refl_equal _)).
+unfold programMaximumMemoryResidence, dropFrame.
+destruct (DropFrame_chk z) as [[[l0 ctx0] ->] |];[cbn|discriminate].
+inversion_clear 1.
+set (z0 := Build_State _ _ _ _) in Hty |- *.
+unfold MemoryBound in *; cbn.
+unfold stateSize.
+rewrite <- Hsx, <- Hty.
+fold (stateSize y0); fold (stateSize ctx0); fold (stateSize x0); fold (stateSize x).
+rewrite N.add_assoc.
+replace (stateSize x + _) with (stateSize x0).
+ rewrite <- N.add_max_distr_l,
+         (N.max_l (stateSize y0) (stateSize ctx0)),
+         (N.max_r (stateSize x) (stateSize x0)),
+         (N.max_comm nx _), (N.max_assoc (stateSize x0) _ _), N.max_id,
+         N.max_assoc, N.max_comm.
+   replace (stateSize y0) with (stateSize x0) in *.
+    apply N.max_le_compat; apply N.max_lub; solve [assumption|apply N.le_add_r].
+   clear -Hsx.
+   unfold stateSize.
+   rewrite Hsx.
+   unfold y, y0, stateShape, stateShapeSize; cbn.
+   rewrite fullWriteFrame_size.
+   ring.
+  unfold x0; clear.
+  destruct x as [irf arf awf iwf]; cbn.
+  unfold stateSize, stateShape, stateShapeSize; cbn.
+  repeat rewrite N.add_assoc; repeat apply N.add_le_mono_r.
+  repeat rewrite <- N.add_assoc; repeat apply N.add_le_mono_l.
+  apply N.le_add_r.
+ unfold stateSize.
+ rewrite Hty.
+ unfold z0; clear.
+ destruct ctx0 as [irf arf awf iwf]; cbn.
+ unfold stateShape, stateShapeSize; cbn.
+ repeat rewrite N.add_assoc; repeat apply N.add_le_mono_r.
+ rewrite N.add_comm.
+ apply N.le_add_r.
+unfold x0; clear.
+destruct x as [irf arf awf iwf]; cbn.
+unfold stateSize, stateShape, stateShapeSize; cbn.
+ring.
+Qed.
+
+Lemma unit_spec {A : Ty} : spec (@unit A).
+Proof.
+intros x n; unfold MemoryBound; cbn.
+inversion_clear 1.
+rewrite N.add_0_r.
+reflexivity.
+Qed.
+
+Lemma injl_spec {A B C : Ty} (t : Term A B) :
+ spec t -> spec (@injl A B C t).
+Proof.
+intros Ht x n; cbn.
+repeat rewrite pMMR_seq.
+repeat rewrite runMachine_seq.
+rewrite pMMR_write.
+assert (Hx := stateShape_write false x).
+destruct (runMachine _ x) as [x0|];[cbn|discriminate].
+specialize (Hx _ (refl_equal _)).
+rewrite pMMR_skip.
+assert (Hx0 := stateShape_skip (padL B C) x0).
+destruct (runMachine _ x0) as [x1|];[cbn|discriminate].
+specialize (Hx0 _ (refl_equal _)).
+specialize (Ht x1).
+destruct (programMaximumMemoryResidence _ x1) as [nt|];[cbn|discriminate].
+specialize (Ht _ (refl_equal _)).
+inversion_clear 1.
+unfold MemoryBound, stateSize in *; cbn.
+rewrite Hx, Hx0; clear -Ht.
+rewrite N.max_id.
+apply N.max_lub;[assumption|].
+apply N.le_add_r.
+Qed.
+
+Lemma injr_spec {A B C : Ty} (t : Term A C) :
+ spec t -> spec (@injr A B C t).
+Proof.
+intros Ht x n; cbn.
+repeat rewrite pMMR_seq.
+repeat rewrite runMachine_seq.
+rewrite pMMR_write.
+assert (Hx := stateShape_write true x).
+destruct (runMachine _ x) as [x0|];[cbn|discriminate].
+specialize (Hx _ (refl_equal _)).
+rewrite pMMR_skip.
+assert (Hx0 := stateShape_skip (padR B C) x0).
+destruct (runMachine _ x0) as [x1|];[cbn|discriminate].
+specialize (Hx0 _ (refl_equal _)).
+specialize (Ht x1).
+destruct (programMaximumMemoryResidence _ x1) as [nt|];[cbn|discriminate].
+specialize (Ht _ (refl_equal _)).
+inversion_clear 1.
+unfold MemoryBound, stateSize in *; cbn.
+rewrite Hx, Hx0; clear -Ht.
+rewrite N.max_id.
+apply N.max_lub;[assumption|].
+apply N.le_add_r.
+Qed.
+
+Lemma bump_spec {A B : Ty} (t : Term A B) (Ht : spec t) :
+ forall x n m, programMaximumMemoryResidence (bump n (@Core.eval _ _ t Naive.translate)) x = Some m ->
+               m <= MemoryBound t x.
+Proof.
+intros x n m.
+unfold bump.
+repeat rewrite pMMR_seq.
+repeat rewrite runMachine_seq.
+rewrite pMMR_fwd.
+assert (Hx := stateShape_fwd n x).
+destruct (runMachine _ x) as [x0|];[cbn|discriminate].
+specialize (Hx _ (refl_equal _)).
+specialize (Ht x0).
+unfold programMaximumMemoryResidence in Ht.
+unfold programMaximumMemoryResidence at 2.
+unfold runMachine.
+destruct (Core.eval _) as [[y tr0] |];[cbn in *|discriminate].
+specialize (Ht _ (refl_equal _)).
+rewrite pMMR_bwd.
+assert (Hy := stateShape_bwd n y).
+destruct (runMachine _ y) as [y0|];[cbn|discriminate].
+specialize (Hy _ (refl_equal _)).
+inversion_clear 1.
+unfold MemoryBound, stateSize.
+rewrite Hx.
+etransitivity;[|apply Ht].
+rewrite N.max_comm, <- N.max_assoc.
+apply N.max_lub;[reflexivity|apply MMR_bounds].
+Qed.
+
+Lemma case_spec {A B C D : Ty} (s : Term (A * C) D) (t : Term (B * C) D) :
+ spec s -> spec t -> spec (case s t).
+Proof.
+intros Hs Ht x n; cbn.
+unfold MemoryBound; cbn.
+rewrite pMMR_choice.
+rewrite <- N.add_max_distr_l.
+destruct (nextData _) as [| [[|] |] _]; try discriminate;
+ intros Hp;etransitivity;[|apply N.le_max_r| |apply N.le_max_l];
+ revert Hp;apply bump_spec; assumption.
+Qed.
+
+Lemma pair_spec {A B C : Ty} (s : Term A B) (t : Term A C) :
+ spec s -> spec t -> spec (pair s t).
+Proof.
+intros Hs Ht x n; unfold MemoryBound; cbn.
+rewrite pMMR_seq.
+specialize (Hs x).
+destruct (programMaximumMemoryResidence _ x) as [ns|];[cbn|discriminate].
+specialize (Hs _ (refl_equal _)).
+assert (Hsx := StateShape.Core_spec s x).
+destruct (runMachine _ x) as [y|];[cbn|discriminate].
+specialize (Hsx _ (refl_equal _)).
+specialize (Ht y).
+destruct (programMaximumMemoryResidence _ y) as [nt|];[cbn|discriminate].
+specialize (Ht _ (refl_equal _)).
+inversion_clear 1.
+rewrite N.max_comm.
+transitivity (N.max (MemoryBound s x) (MemoryBound t y)).
+ apply N.max_le_compat; assumption.
+unfold MemoryBound, stateSize.
+rewrite Hsx, N.add_max_distr_l.
+reflexivity.
+Qed.
+
+Lemma take_spec {A B C : Ty} (t : Term A C) :
+ spec t -> spec (@take A B C t).
+Proof.
+auto.
+Qed.
+
+Lemma drop_spec {A B C : Ty} (t : Term B C) :
+ spec t -> spec (@drop A B C t).
+Proof.
+intros Ht x n Hp;cbn.
+apply (bump_spec _ Ht _ _ _ Hp).
+Qed.
+
+Lemma Core_spec {A B : Ty} (t : Term A B) :
+ spec t.
+Proof.
+induction t.
+- apply iden_spec.
+- apply comp_spec; assumption.
+- apply unit_spec.
+- apply injl_spec; assumption.
+- apply injr_spec; assumption.
+- apply case_spec; assumption.
+- apply pair_spec; assumption.
+- apply take_spec; assumption.
+- apply drop_spec; assumption.
+Qed.
+
+Definition CellBound {A B : Ty} (t : Term A B) : N := N.of_nat (bitSize A) + N.of_nat (bitSize B) + (@Core.eval _ _ t extraMemoryBound).
+
+Lemma CellBound_correct {A B : Ty} (t : Term A B) a n:
+  programMaximumMemoryResidence (@Core.eval _ _ t Naive.translate) (fillContext emptyCtx (LocalStateBegin t a)) = Some n ->
+  n <= CellBound t.
+Proof.
+intros Ht.
+etransitivity;[apply (Core_spec _ _ _ Ht)|].
+unfold MemoryBound, CellBound, stateSize, stateShapeSize; cbn.
+rewrite app_nil_r, encode_length, N.add_0_r, <- plus_n_O.
+reflexivity.
+Qed.
+
+End MaximumMemory.
